VCG.thy
@@ -16,6 +16,81 @@ lemma hoare_intro:
 
 
 
+section "Annotations"
+
+type_synonym block_preconditions = "(llvm_label * (state \<Rightarrow> bool)) list"
+type_synonym function_postcondition = "(llvm_value * state) \<Rightarrow> bool"
+datatype annotated_function = annotated "llvm_function" "block_preconditions" "function_postcondition"
+
+partial_function (tailrec) execute_blocks_from_until :: "annotated_function \<Rightarrow> llvm_label \<Rightarrow> llvm_label option \<Rightarrow> state \<Rightarrow> (state * llvm_block_return) result" where
+  "execute_blocks_from_until fun label prev s = (case fun of annotated (func fdef blocks) pre post \<Rightarrow>
+    (case map_of blocks label of
+      None \<Rightarrow> err unknown_label
+    | Some b \<Rightarrow> (case (execute_block prev b s) of
+        ok (s', return_value v) \<Rightarrow> ok (s', return_value v)
+      | ok (s', branch_label l) \<Rightarrow> (case map_of pre l of
+          Some _ \<Rightarrow> ok (s', branch_label l)
+        | None \<Rightarrow> execute_blocks_from_until fun l (Some label) s'
+        )
+      | err e \<Rightarrow> err e
+      )
+    )
+  )"
+lemmas [code] = execute_blocks_from_until.simps
+
+
+lemma hoare_blocks_from_until_intro:
+  assumes "map_of blocks label = Some b"
+  assumes "hoare
+            P
+            (execute_block prev b)
+            (\<lambda>(s, r). case r of
+              return_value v \<Rightarrow> Q (s, r)
+            | branch_label l \<Rightarrow> (case map_of pre l of
+                Some _ \<Rightarrow> Q (s, r)
+              | None \<Rightarrow>
+                hoare
+                  (\<lambda>s'. s' = s)
+                  (execute_blocks_from_until (annotated (func fdef blocks) pre post) l (Some label))
+                Q
+              )
+            )"
+  shows "hoare P (execute_blocks_from_until (annotated (func fdef blocks) pre post) label prev) Q"
+  apply (rule hoare_intro)
+  using assms
+  apply (auto simp: execute_blocks_from_until.simps)
+  subgoal for r s h
+  unfolding hoare_def wp_gen_def
+  apply (cases "execute_block prev b (r, s, h)")
+  apply auto
+  subgoal for r' s' h' ret
+    apply (cases ret)
+     apply auto apply force
+    subgoal for l 
+      apply (cases "map_of pre l") apply auto apply force by fastforce
+    done
+  by fastforce
+  done
+
+fun verify_from_with_precond where
+  "verify_from_with_precond (annotated (func fdef blocks) pre post) label precond =
+    hoare
+      precond
+      (execute_blocks_from_until (annotated (func fdef blocks) pre post) label None)
+      (\<lambda>(s, r). (case r of
+        return_value v \<Rightarrow> post (v, s)
+      | branch_label l \<Rightarrow> (case map_of pre l of
+          Some Q \<Rightarrow> Q s
+        | None \<Rightarrow> False
+        )
+      ))"
+
+fun verify_from where
+  "verify_from (annotated f pre post) label = (case map_of pre label of
+    Some precond \<Rightarrow> verify_from_with_precond (annotated f pre post) label precond
+  | None \<Rightarrow> verify_from_with_precond (annotated f pre post) label (\<lambda>s. True))"
+
+
 section "Useful Lemmas"
 
 lemma contract_updates:
@@ -48,55 +123,91 @@ method clean_memory = repeat_minus_one thin_tac_mem
 method clean_assms = ((elim exE conjE)+)?, (simp only: contract_updates)?; clean_registers?; clean_memory?; (simp only: triv_forall_equality)?
 
 
-subsection "Specific Subgoal Methods"
+subsection "Subgoal Solving Methods"
 
-method instantiate_register_address = rule asm_rl[of "register_\<alpha> _ _ = Some (addr _)"]; simp
-method memory_allocated = rule asm_rl[of "memory_\<alpha> _ _ \<noteq> None"]; simp
-method register_value = rule asm_rl[of "register_\<alpha> _ _ = Some _"]; simp
-method memory_value = rule asm_rl[of "memory_\<alpha> _ _ = Some (Some _)"]; simp split: if_splits
-method add_poison = (rule asm_rl[of "add_no_poison32 _ _ _"] | rule asm_rl[of "add_no_poison64 _ _ _"]); eval
-method icmp_same_signs = rule asm_rl[of "if _ then same_signs _ _ else True"]; eval
-method map_of_some = rule asm_rl[of "map_of _ _ = Some _"]; simp
-method distinct_first = rule asm_rl[of "distinct (map fst _)"]; eval
-method some_refl = rule asm_rl[of "Some _ = Some _"]; rule refl
+method sub_instantiate_register_address = rule asm_rl[of "register_\<alpha> _ _ = Some (addr _)"]; (fastforce | simp); fail
+method sub_memory_allocated = rule asm_rl[of "memory_\<alpha> _ _ \<noteq> None"]; (fastforce | simp); fail
+method sub_register_value = rule asm_rl[of "register_\<alpha> _ _ = Some _"]; (fastforce | simp); fail
+method sub_memory_value = rule asm_rl[of "memory_\<alpha> _ _ = Some (Some _)"]; (fastforce | simp split: if_splits); fail
+method sub_add_poison = (rule asm_rl[of "add_no_poison32 _ _ _"] | rule asm_rl[of "add_no_poison64 _ _ _"]); (fastforce | simp); fail
+method sub_icmp_same_signs = rule asm_rl[of "if _ then same_signs _ _ else True"]; (fastforce | simp); fail
+method sub_map_of_some = rule asm_rl[of "map_of _ _ = Some _"]; (fastforce | simp); fail
+method sub_distinct_first = rule asm_rl[of "distinct (map fst _)"]; (fastforce | simp); fail
+method sub_some_refl = rule asm_rl[of "Some _ = Some _"]; rule refl; fail
+
+method solve_subgoal = sub_instantiate_register_address | sub_memory_allocated | sub_register_value
+                     | sub_memory_value | sub_add_poison | sub_icmp_same_signs | sub_map_of_some
+                     | sub_distinct_first | sub_some_refl
 
 
 subsection "Instruction Methods"
 
 method strat_instr methods m = rule wp_intro, m, clean_assms; (simp only: False_eq_False)?
+method strat_instr_dbg = (rule wp_intro, (solve_subgoal+)?); (rule asm_rl[of "wp _ _"], clean_assms)?; (simp only: False_eq_False)?
 
 method strat_alloca = rule asm_rl[of "wp (execute_alloca _ _) _"], strat_instr -
-method strat_store  = rule asm_rl[of "wp (execute_store _ _ _) _"], strat_instr \<open>instantiate_register_address, memory_allocated, register_value\<close>
-method strat_load   = rule asm_rl[of "wp (execute_load _ _ _) _"], strat_instr \<open>instantiate_register_address, memory_value\<close>
-method strat_add    = rule asm_rl[of "wp (execute_add _ _ _ _ _) _"], strat_instr \<open>register_value, register_value, add_poison\<close>
-method strat_icmp   = rule asm_rl[of "wp (execute_icmp _ _ _ _ _ _) _"], strat_instr \<open>register_value, register_value, icmp_same_signs\<close>; simp only: compare_values_32.simps compare_values_64.simps
+method strat_store  = rule asm_rl[of "wp (execute_store _ _ _) _"], strat_instr \<open>sub_instantiate_register_address, sub_memory_allocated, sub_register_value\<close>
+method strat_load   = rule asm_rl[of "wp (execute_load _ _ _) _"], strat_instr \<open>sub_instantiate_register_address, sub_memory_value\<close>
+method strat_add    = rule asm_rl[of "wp (execute_add _ _ _ _ _) _"], strat_instr \<open>sub_register_value, sub_register_value, sub_add_poison\<close>
+method strat_icmp   = rule asm_rl[of "wp (execute_icmp _ _ _ _ _ _) _"], strat_instr \<open>sub_register_value, sub_register_value, sub_icmp_same_signs\<close>; simp only: compare_values_32.simps compare_values_64.simps
+
+method strat_alloca_dbg = rule asm_rl[of "wp (execute_alloca _ _) _"], strat_instr_dbg
+method strat_store_dbg  = rule asm_rl[of "wp (execute_store _ _ _) _"], strat_instr_dbg
+method strat_load_dbg   = rule asm_rl[of "wp (execute_load _ _ _) _"], strat_instr_dbg
+method strat_add_dbg    = rule asm_rl[of "wp (execute_add _ _ _ _ _) _"], strat_instr_dbg
+method strat_icmp_dbg   = rule asm_rl[of "wp (execute_icmp _ _ _ _ _ _) _"], strat_instr_dbg; simp only: compare_values_32.simps compare_values_64.simps
 
 method unfold_block_instr = rule asm_rl[of "wp (execute_block _ ([], _#_, _) _) _"], rule wp_intro
 method unfold_instr = rule asm_rl[of "wp (execute_instruction _ _) _"], rule wp_intro
 
-method instr_vcg = (unfold_block_instr | unfold_instr | strat_alloca | strat_store | strat_load | strat_add | strat_icmp)+
+method instr_vcg_step = unfold_block_instr | unfold_instr | strat_alloca | strat_store | strat_load | strat_add | strat_icmp
+method instr_vcg_step_dbg = unfold_block_instr | unfold_instr | strat_alloca_dbg | strat_store_dbg | strat_load_dbg | strat_add_dbg | strat_icmp_dbg
 
 
 subsection "Phi Node Methods"
 
-method strat_phi = rule asm_rl[of "wp (execute_phi _ _ _ _) _"], strat_instr \<open>distinct_first, some_refl, map_of_some, register_value\<close>
+method strat_phi = rule asm_rl[of "wp (execute_phi _ _ _ _) _"], strat_instr \<open>sub_distinct_first, sub_some_refl, sub_map_of_some, sub_register_value\<close>
+method strat_phi_dbg = rule asm_rl[of "wp (execute_phi _ _ _ _) _"], strat_instr_dbg
 
 method unfold_block_phi = rule asm_rl[of "wp (execute_block _ (_#_, _, _) _) _"], rule wp_intro
 
-method phi_vcg = (unfold_block_phi | strat_phi)+
+method phi_vcg_step = unfold_block_phi | strat_phi
+method phi_vcg_step_dbg = unfold_block_phi | strat_phi_dbg
 
 
 subsection "Terminal Instruction Methods"
 
-method strat_branch_i1 = rule asm_rl[of "wp (execute_block _ ([], [], br_i1 _ _ _) _ ) _"], (rule wp_intro, register_value); (simp only: False_eq_False)?
+method strat_branch_i1 = rule asm_rl[of "wp (execute_block _ ([], [], br_i1 _ _ _) _ ) _"], (rule wp_intro, sub_register_value); (simp only: False_eq_False)?
 method strat_branch_label = rule asm_rl[of "wp (execute_block _ ([], [], br_label _) _ ) _"], rule wp_intro; (simp only: False_eq_False)?
-method strat_return = rule asm_rl[of "wp (execute_block _ ([], [], ret _ _) _ ) _"], (rule wp_intro, register_value); (simp only: False_eq_False)?
+method strat_return = rule asm_rl[of "wp (execute_block _ ([], [], ret _ _) _ ) _"], (rule wp_intro, sub_register_value); (simp only: False_eq_False)?
 
-method term_vcg = strat_branch_i1 | strat_branch_label | strat_return
+method term_vcg_step_dbg = rule asm_rl[of "wp (execute_block _ ([], [], _) _) _"], rule wp_intro, (solve_subgoal+)?; (simp only: False_eq_False)?
+
+method term_vcg_step = strat_branch_i1 | strat_branch_label | strat_return
 
 
-subsection "VCG Method"
+subsection "Block VCG Methods"
 
-method vcg = rule hoare_intro, phi_vcg?, instr_vcg?, term_vcg?
+method unfold_hoare = rule asm_rl[of "hoare _ (execute_block _ _) _"], rule hoare_intro
+
+method block_vcg_step = unfold_hoare | phi_vcg_step | instr_vcg_step | term_vcg_step
+method block_vcg_step_dbg = unfold_hoare | phi_vcg_step_dbg | instr_vcg_step_dbg | term_vcg_step_dbg
+
+method block_vcg = block_vcg_step+
+method block_vcg_dbg = block_vcg_step_dbg+
+
+
+subsection "Multi-Block VCG Methods"
+
+method clean_goal = rule asm_rl[of "case _ of _ \<Rightarrow> (case _ of _ \<Rightarrow> _)"]
+                  , auto simp only: split prod.case split: llvm_block_return.splits option.splits if_splits; (simp; fail)?
+
+method unfold_execute_blocks_from_until = rule asm_rl[of "hoare _ (execute_blocks_from_until _ _ _) _"], rule hoare_blocks_from_until_intro, sub_map_of_some
+method unfold_verify = rule asm_rl[of "verify_from _ _"], simp
+
+method vcg_step = unfold_verify | unfold_execute_blocks_from_until | block_vcg_step
+method vcg_step_dbg = unfold_verify | unfold_execute_blocks_from_until | block_vcg_step_dbg 
+method vcg = vcg_step+
+method vcg_dbg = vcg_step_dbg+
 
 end
